-

coq/Series.v
@@ -1,11 +1,11 @@
-(* $Id: Series.v,v 1.10 2013-06-19 16:29:38 deraugla Exp $ *)
+(* $Id: Series.v,v 1.11 2013-06-20 07:28:46 deraugla Exp $ *)
 
 Require Import Utf8.
 
 Set Implicit Arguments.
 
-Inductive series α :=
-  | Term : α → (unit → series α) → series α
+CoInductive series α :=
+  | Term : α → series α → series α
   | End : series α.
 
 Definition series_hd α (s : series α) :=
@@ -16,7 +16,7 @@ Definition series_hd α (s : series α) :=
 
 Definition series_tl α (s : series α) : option (series α) :=
   match s with
-  | Term _ t => Some (t tt)
+  | Term _ t => Some t
   | End => None
   end.
 
@@ -36,9 +36,9 @@ Definition series_nth α (n : nat) (s : series α) : option α :=
   | Some t => series_hd t
   end.
 
-Fixpoint series_map α β (f : α → β) s :=
+CoFixpoint series_map α β (f : α → β) s :=
   match s with
-  | Term a t => Term (f a) (λ tt, series_map f (t tt))
+  | Term a t => Term (f a) (series_map f t)
   | End => End _
   end.
 
@@ -49,15 +49,15 @@ intros α s.
 destruct s; reflexivity.
 Qed.
 
-Inductive series_forall α P (s : series α) : Prop :=
+CoInductive series_forall α P (s : series α) : Prop :=
   | TermAndFurther : ∀ a t,
-      s = Term a t → P a → series_forall P (t tt) → series_forall P s
+      s = Term a t → P a → series_forall P t → series_forall P s
   | EndOk :
       s = End _ → series_forall P s.
 
 Lemma series_forall_inv : ∀ α (P : α → Prop) t s,
   series_forall P (Term t s)
-  → P t ∧ series_forall P (s tt).
+  → P t ∧ series_forall P s.
 Proof.
 intros α P t s H.
 inversion H; [ idtac | discriminate H0 ].
@@ -67,8 +67,9 @@ Qed.
 Lemma series_forall_map : ∀ α (P Q : _ → Prop) (s : series α),
   (∀ x, P x → Q x) → series_forall P s → series_forall Q s.
 Proof.
+cofix IHs.
 intros α P Q s Hx H.
-induction s as [t₁ s₁ IHs| ].
+destruct s as [t₁ s₁| ].
  apply series_forall_inv in H.
  destruct H as (H₁, H₂).
  eapply TermAndFurther; [ reflexivity | apply Hx, H₁ | idtac ].
